% !TEX root= ../main.tex
\section{Proving inconsistency of unrestricted theories}
\label{sec:Proving inconsistency of unrestricted theories}
This section will show that there exist inconsistencies in non-graph-based theories that are not possible to prove in Neg using only unary and binary NAND-clauses.
We will prove the pigeonhole principle to examplify this.

The pigeonhole principle states that whenever you have $n$ pigeons and $m$ holes such that $n > m$, then at least one hole must contain more than one pigeon.
We can prove this principle in Neg by proving an inconsistency in the theory that (1) all $n$ pigeons are contained in a hole and (2) each hole contains only one pigeon.

Letting the atom $x_i$ denote the pigeon $i$ occupying the hole $x$, the above theory, with $n$ pigeons and $m$ holes, can be formalized in the following way:
\begin{align}
  \text{(1):}\quad &\{ \; 1_i2_i3_i\dots m_i \;|\; i \leq n \; \}\\
  \text{(2):}\quad &\{ \; x_ix_j \;|\; i < j \leq n, x \leq m \; \}
\end{align}
\subsection{Proving the pigeonhole principle - 4 pigeons, 3 holes}
\label{sub:Proving the pigeonhole principle - 4 pigeons, 3 holes}
The pigeonhole principle for 4 pigeons and 3 holes will have the following axioms:
\begin{align}
  \text{OR} &= \{ \; 1_12_13_1,\; 1_22_23_2,\; 1_32_33_3,\; 1_42_43_4 \; \}\\
  \text{NAND} &= \left \{
  \begin{tabular}{c}
    $\ol{1_11_2},\;\ol{1_11_3},\;\ol{1_11_4},\;\ol{1_21_3},\;\ol{1_21_4},\;\ol{1_31_4},$\\
    $\ol{2_12_2},\;\ol{2_12_3},\;\ol{2_12_4},\;\ol{2_22_3},\;\ol{2_22_4},\;\ol{2_32_4},$\\
    $\ol{3_12_2},\;\ol{3_13_3},\;\ol{3_13_4},\;\ol{3_23_3},\;\ol{3_23_4},\;\ol{3_33_4}$
  \end{tabular}
  \right \}
\end{align}

From the axioms above we can prove inconsistency in the following way:

Proving $\ol{1_4}$:
\begin{prooftree*}[separation=0.8em, rule margin=1ex]
  \Hypo{\ol{1_31_4}}
    \Hypo{\ol{1_21_4}}
    \Hypo{\ol{2_22_3}}
      \Hypo{\ol{1_11_4}}
      \Hypo{\ol{2_12_3}}
      \Hypo{\ol{3_13_2}}
    \Infer[right label = $1_12_13_1$]3{\ol{3_22_31_4}}
  \Infer[right label = $1_22_23_2$]3{\ol{2_31_4}}
    \Hypo{\ol{1_21_4}}
      \Hypo{\ol{1_11_4}}
      \Hypo{\ol{2_12_2}}
      \Hypo{\ol{3_13_3}}
    \Infer[right label = $1_12_13_1$]3{\ol{2_23_31_4}}
    \Hypo{\ol{3_23_3}}
  \Infer[right label = $1_22_23_2$]3{\ol{3_31_4}}
\Infer[right label = $1_32_33_3$, separation=0em]3{\ol{1_4}}
\end{prooftree*}

Proving $\ol{2_4}$:
\begin{prooftree*}[separation=0.8em, rule margin=1ex]
    \Hypo{\ol{1_21_3}}
    \Hypo{\ol{2_22_4}}
      \Hypo{\ol{1_11_3}}
      \Hypo{\ol{2_12_4}}
      \Hypo{\ol{3_13_2}}
    \Infer[right label = $1_12_13_1$]3{\ol{3_21_32_4}}
  \Infer[right label = $1_22_23_2$]3{\ol{1_32_4}}
  \Hypo{\ol{2_32_4}}
      \Hypo{\ol{1_11_2}}
      \Hypo{\ol{2_12_4}}
      \Hypo{\ol{3_13_3}}
    \Infer[left label = $1_12_13_1$]3{\ol{1_23_32_4}}
    \Hypo{\ol{2_22_4}}
    \Hypo{\ol{3_23_3}}
  \Infer[left label = $1_22_23_2$]3{\ol{3_32_4}}
\Infer[right label = $1_32_33_3$, separation=0em]3{\ol{2_4}}
\end{prooftree*}

Proving $\ol{3_4}$:
\begin{prooftree*}[separation=0.8em, rule margin=1ex]
    \Hypo{\ol{1_21_3}}
      \Hypo{\ol{1_11_3}}
      \Hypo{\ol{2_12_2}}
      \Hypo{\ol{3_13_4}}
    \Infer[left label = $1_12_13_1$]3{\ol{2_21_33_4}}
    \Hypo{\ol{3_23_4}}
  \Infer[left label = $1_22_23_2$]3{\ol{1_33_4}}
      \Hypo{\ol{1_11_2}}
      \Hypo{\ol{2_12_3}}
      \Hypo{\ol{3_13_4}}
    \Infer[left label = $1_12_13_1$]3{\ol{1_22_33_4}}
    \Hypo{\ol{2_22_3}}
    \Hypo{\ol{3_23_4}}
  \Infer[left label = $1_22_23_2$]3{\ol{2_33_4}}
  \Hypo{\ol{3_33_4}}
\Infer[left label = $1_32_33_3$, separation=0em]3{\ol{3_4}}
\end{prooftree*}

With these three unary clauses proven, we can now prove $\varnothing$ in one step:
\begin{prooftree*}[rule margin=1ex]
  \Hypo{\ol{1_4}}
  \Hypo{\ol{2_4}}
  \Hypo{\ol{3_4}}
  \Infer[left label = $1_42_43_4$]3{\varnothing}
\end{prooftree*}
