% !TEX root= ../main.tex
\section{Unary NAND-clauses in graph theories}
\label{sec:Unary NAND-clauses in graph theories}
We will to use the fact that some binary NAND-clauses are not binary-derivable to show that some \textit{unary} NAND-clauses are not binary-derivable.

In order to do this, we will first prove a lemma.

Let $G$ and $H$ be two graphs with vertices $v_G \in G$ and $v_H \in H$.
Let $x$ be a vertex such that both $v_G \in N(x)$ and $v_H \in N(x)$
\begin{lemma}
  If
\end{lemma}

Consider the following extension to our original graph from Figure~\ref{fig:open_door}:
\[
  \begin{tikzpicture}
    [
    point/.style={circle,draw,inner sep=0pt,minimum size=2mm},
    collection/.style={thick,rectangle,draw,inner sep=0pt,minimum height=14mm, minimum width= 9mm}
    ]
    \node (a) at (0,2) [point,label=left:$a$] {};
    \node (x1) at (0,4) [point,label=left:$x_1$] {};
    \node (x2) at (0,0) [point,label=left:$x_2$] {};
    \node (b) at (2,2) [point,label=right:$b$] {};
    \node (y1) at (2,4) [point,label=right:$y_1$] {};
    \node (y2) at (2,0) [point,label=right:$y_2$] {};
    \node (c1) at (1,3) [point,label=right:$c_1$] {};
    \node (c2) at (1,1) [point,label=right:$c_2$] {};
    \node (s) at (1,6) [point,label=left:$s$] {};
    \node (t) at (1,5) [point,label=below:$t$] {};
    \node (u1) at (-2,5) [point,label=left:$u_1$] {};
    \node (u2) at (4,5) [point,label=right:$u_2$] {};
    \draw [-latex] (a) to (x1);
    \draw [-latex] (a) to (x2);
    \draw [-latex] (b) to (y1);
    \draw [-latex] (b) to (y2);
    \draw [-latex] (x1) to (y1);
    \draw [-latex] (x1) to (c1);
    \draw [-latex] (x2) to (y2);
    \draw [-latex] (x2) to (c2);
    \draw [-latex] (c1) to (c2);
    \draw [-latex,loop right] (s) to (s);
    \draw [-latex] (s) to (t);
    \draw [-latex] (t) to (u1);
    \draw [-latex] (t) to (u2);
    \draw [-latex] (u1) to (a);
    \draw [-latex] (u2) to (b);
  \end{tikzpicture}
\]
The extension provides us with 6 new NAND-clauses and 4 new OR-clauses in the axioms set:
\begin{align}
  \text{OR'} &= \text{OR} \cup \{st,\; tu_1u_2,\; u_1a,\; u_2b \}\\
  \text{NAND'} &= \text{NAND} \cup \{\ol{s},\; \ol{st},\; \ol{tu_1},\; \ol{tu_2},\; \ol{u_1a},\; \ol{u_2b} \}
\end{align}
This extended graph can now be proven inconsistent using the newly provided clauses, as shown in the following Neg proof:
\begin{prooftree*}
  \Hypo{\ol{s}}
  \Hypo{\ol{tu_2}}
  \Hypo{\ol{tu_1}}
  \Hypo{\dots}
  \Infer1{\ol{ab}}
  \Infer[right label=$u_1a$]2{\ol{tb}}
  \Infer[right label=$u_2b$]2{\ol{t}}
  \Infer[right label=$st$]2{\varnothing}
\end{prooftree*}
Since $\ol{ab}$ needs a non-binary proof, the above proof is non-binary.

One could think of this proof to be working ``bottom up'' from the proved statement $\ol{ab}$.
The argumentation of the above inconsistency proof can informally be presented like this:
\begin{enumerate}
  \item $a$ and $b$ cannot both be 1
  \item $\Rightarrow$ $u_1$ and $u_2$ cannot both be 0
  \item $\Rightarrow$ $t$ cannot be 1
  \item $\Rightarrow$ $s$ cannot be 0, but $s$ has to be 0
\end{enumerate}
